PivotBetree/Bounds.i.dfy
@@ -9,7 +9,9 @@ module Bounds {
   import opened NativeTypes
   import opened KeyType
 
-  function method BlockSizeUint64() : uint64 { 8*1024*1024 }
+  function method IndirectionTableBlockSizeUint64() : uint64 { 8*1024*1024 }
+  function method NodeBlockSizeUint64() : uint64 { 98304 }
+  function method MinNodeBlockIndexUint64() : uint64 { 86 }
 
   //function method MaxTotalBucketWeightUint64() : uint64 { 8356168 }
   //function method MaxCacheSizeUint64() : uint64 { 200 }
@@ -25,13 +27,21 @@ module Bounds {
 
   function method IndirectionTableMaxSizeUint64() : uint64 { 0x1_0000_0000 }
 
-  function BlockSize() : int { BlockSizeUint64() as int }
+  function IndirectionTableBlockSize() : int { IndirectionTableBlockSizeUint64() as int }
+  function NodeBlockSize() : int { NodeBlockSizeUint64() as int }
+  function MinNodeBlockIndex() : int { MinNodeBlockIndexUint64() as int }
   function MaxNumChildren() : int { MaxNumChildrenUint64() as int }
   function MaxTotalBucketWeight() : int { MaxTotalBucketWeightUint64() as int }
   function MaxCacheSize() : int { MaxCacheSizeUint64() as int }
   function FlushTriggerWeight() : int { FlushTriggerWeightUint64() as int }
   function NumBlocks() : int { NumBlocksUint64() as int }
   function IndirectionTableMaxSize() : int { IndirectionTableMaxSizeUint64() as int }
+
+  lemma lemma_node_sector_doesnt_overlap_indirection_table()
+  ensures NodeBlockSize() * MinNodeBlockIndex()
+       >= IndirectionTableBlockSize()
+  {
+  }
 
   lemma lemma_node_fits_in_block()
   ensures 32 // checksum
@@ -41,7 +51,7 @@ module Bounds {
     + 8 // number of buckets
     + MaxNumChildren() * (4 + 4) // length of each bucket
     + MaxTotalBucketWeight()
-    == BlockSize()
+    <= NodeBlockSize()
   {
   }
 }
